
\input{high-level}

\subsection{Low Level System}

\subsubsection{Match}

\[
\infer[ok]
{\mo \Delta, p ; \Xi; p, \Omega; H; C \rightarrow \Xi'; \Delta'}
{\mo \Delta; \Xi, p; \Omega; H; C \rightarrow \Xi'; \Delta'}
\tab
\infer[fail]
{\mo \Delta; \Xi; p, \Omega; H; C \rightarrow \Xi'; \Delta'}
{p \notin \Delta & \cont C ; H; \Xi'; \Delta'}
\]

\[
\infer[\tensor]
{\mo \Delta; \Xi; A \otimes B, \Omega ; H ; C \rightarrow \Xi'; \Delta'}
{\mo \Delta; \Xi; A, B, \Omega; H; C \rightarrow \Xi';\Delta'}
\]

\[
\infer[\m{rule} \; \m{cont}]
{\mo \Delta; \Xi; \cdot ; H; (\Phi; \Delta'') \rightarrow \Xi'; \Delta'}
{\done \Delta; \Xi; \cdot ; H; \cdot \rightarrow \Xi'; \Delta'}
\]

\subsubsection{Derive}

\[
\infer[p]
{\done \Delta; \Xi; \Delta_1; p, \Omega; C \rightarrow \Xi'; \Delta'}
{\done \Delta; \Xi; p, \Delta_1; \Omega; C \rightarrow \Xi'; \Delta'}
\tab
\infer[1]
{\done \Delta; \Xi; \Delta_1; 1, \Omega; C \rightarrow \Xi';\Delta'}
{\done \Delta; \Xi; \Delta_1; \Omega; C \rightarrow \Xi'; \Delta'}
\]

\[
\infer[\otimes]
{\done \Delta; \Xi; \Delta_1; A \otimes B, \Omega; C \rightarrow \Xi'; \Delta'}
{\done \Delta; \Xi; \Delta_1; A, B, \Omega; C \rightarrow \Xi';\Delta'}
\]

\[
\infer[\m{comp}]
{\done \Delta; \Xi; \Delta_1; \m{comp} \; A \lolli B, \Omega; \cdot \rightarrow \Xi'; \Delta'}
{\ao \Delta; A \lolli B; (\done \Delta; \Xi; \Delta_1; \m{comp} \; A \lolli B, \Omega; \cdot) \rightarrow \Xi'; \Delta'}
\]

\[
\infer[\m{comp \; derivation}]
{\mo \Delta; \Xi; \cdot; H; (\done \Delta''; \Xi''; \Delta_1; \m{comp} \; A \lolli B, \Omega; \cdot) \rightarrow \Xi'; \Delta'}
{\done \Delta; \Xi; \cdot ; H; (\done \Delta''; \Xi''; \Delta_1; \m{comp} \; A \lolli B, \Omega; \cdot) \rightarrow \Xi'; \Delta'}
\]

\[
\infer[\m{end}]
{\done \Delta; \Xi; \Delta_1; \cdot; \cdot \rightarrow \Xi; \Delta_1}
{}
\]

\[
\infer[\m{next \; comp}]
{\done \Delta; \Xi; \Delta_1; \cdot; (\done \Delta''; \Xi''; \Delta''_1; \m{comp} \; A \lolli B, \Omega) \rightarrow \Xi'; \Delta'}
{\done \Delta; \Xi, \Xi''; \Delta_1, \Delta''_1; \m{comp} \; A \lolli B, \Omega; \cdot \rightarrow \Xi'; \Delta'}
\]

\subsubsection{Continuations}

\[
\infer[\m{rule \; fail}]
{\cont (\Phi; \Delta); \Xi'; \Delta'}
{\doo \Delta; \Phi \rightarrow \Xi'; \Delta'}
\]

\[
\infer[\m{comp \; done}]
{\cont (\done \Delta''; \Xi''; \Delta_1; \m{comp} \; A \lolli B, \Omega); \Xi'; \Delta'}
{\done \Delta; \Xi''; \Delta_1; \Omega; \cdot \rightarrow \Xi'; \Delta'}
\]

\subsubsection{Apply}

\[
\infer[\m{apply \; rule}]
{\ao \Delta; A \lolli B; C \rightarrow \Xi'; \Delta'}
{\mo \Delta; \cdot; A; B; C \rightarrow \Xi'; \Delta'}
\]

\[
\infer[\m{pick \; rule}]
{\doo \Delta; R, \Phi \rightarrow \Xi'; \Delta'}
{\ao \Delta; R; (\Phi; \Delta) \rightarrow \Xi';\Delta'}
\]

\subsection{Low level comprehension match succeeds or fails}

If $\mo \Delta'', \Delta_1, ..., \Delta_n; \Xi; \Omega; H; (\done \Delta'''; \Xi''; \Delta_1; \m{comp} \; A \lolli B, \Omega') \rightarrow \Xi'; \Delta'$ then either:

\begin{itemize}
\item $\cont (\done \Delta'''; \Xi''; \Delta_1; \m{comp} \; A \lolli B, \Omega'); \Xi'; \Delta'$ or
\item $\mo \Delta''; \Xi, \Delta_1, ..., \Delta_n' \cdot ; H ; (\done ...) \rightarrow \Xi'; \Delta'$ and $\Omega = \Omega_1, ..., \Omega_n$ where $\mz \Delta_1; \Omega_1 \rightarrow \Delta_1$, ..., $\mz \Delta_n ; \Omega_n \rightarrow \Delta_n$ and $\Delta_1, ..., \Delta_n$ is not empty.
\end{itemize}

It's trivial by induction on the assumption, except the case $p, \Omega$ and $A \otimes B, \Omega$.

\subsection{Low level comprehension gives one match}

If $\mo \Delta'', \Xi''; \cdot; A ; H; (\done \Delta'''; \Xi; \Delta_1; \m{comp} \; A \lolli B, \Omega') \rightarrow \Xi'; \Delta'$ then either

\begin{itemize}
\item $\cont (\done \Delta'''; \Xi; \Delta_1; \m{comp} \; A \lolli B, \Omega'); \Xi'; \Delta'$ or
\item $\mo \Delta'' ; \Xi''; \cdot; H; (\done \Delta'''; \Xi; \Delta_1; \m{comp} \; A \lolli B, \Omega') \rightarrow \Xi'; \Delta'$ and $\mz \Xi''; A \rightarrow \Xi''$, where $\Xi''$ is not empty
\end{itemize}

This follows trivially from the previous theorem.

\subsection{Comprehension head is another derivation theorem}

If $\done \Delta; \Xi; \Delta_1; \Omega'; (\done \Delta''; \Xi''; \Delta'_1; \m{comp} \; A \lolli B, \Omega) \rightarrow \Xi'; \Delta'$ \\ then \\ $\done \Delta; \Xi, \Xi''; \Delta_1, \Delta'_1; \Omega', \m{comp} \; A \lolli B, \Omega; \cdot \rightarrow \Xi'; \Delta'$.

\begin{itemize}
\item $p$

$\done \Delta; \Xi; \Delta_1; p, \Omega''; (\done ...) \rightarrow \Xi'; \Delta'$ \hfill (1) assumption \\
$\Omega' = p, \Omega''$ \hfill (2) from (1) \\
$\done \Delta; \Xi; p, \Delta_1; \Omega''; (\done ...) \rightarrow \Xi'; \Delta'$ \hfill (3) inversion of (1) \\
$\done \Delta; \Xi, \Xi''; p, \Delta_1, \Delta'_1; \Omega'', \m{comp} \; A \lolli B, \Omega; \cdot \rightarrow \Xi'; \Delta'$ \hfill (4) i.h. on (3) \\
$\done \Delta; \Xi, \Xi''; \Delta_1, \Delta'_1; p, \Omega'', \m{comp} \; A \lolli B, \Omega; \cdot \rightarrow \Xi'; \Delta'$ \hfill (5) apply rule on (4) \\

\item $A \otimes B$

$\done \Delta; \Xi, \Xi''; \Delta_1, \Delta'_1; A, B, \Omega''; \m{comp} \; A \lolli B, \Omega; \cdot \rightarrow \Xi'; \Delta'$ \hfill (1) by i.h. \\
$\done \Delta; \Xi, \Xi''; \Delta_1, \Delta'_1; A \otimes B, \Omega''; \m{comp} \; A \lolli B, \Omega; \cdot \rightarrow \Xi'; \Delta'$ \hfill (2) rule application on (1) \\

\item $\cdot$

$\done \Delta; \Xi; \Delta_1; \cdot; (\done \Delta''; \Xi''; \Delta'_1; \m{comp} \; A \lolli B, \Omega) \rightarrow \Xi'; \Delta'$ \hfill (1) assumption \\
$\done \Delta; \Xi, \Xi''; \Delta_1, \Delta'_1; \m{comp} \; A \lolli B, \Omega; \cdot \rightarrow \Xi'; \Delta'$ \hfill (2) inversion of (1) \\

\end{itemize}

\subsection{Low level matching gives high level matching theorem}

If \\
$\mo \Delta, \Delta_1, ..., \Delta_n; \Xi; A_1, ..., A_n; H; \cdot \rightarrow \Xi'; \Delta'$ \\
then \\
$\mz \Delta_1; A_1 \rightarrow \Delta_1$ through $\mz \Delta_n; A_n \rightarrow \Delta_n$ and \\
$\mo \Delta; \Xi, \Delta_1, ..., \Delta_n; \cdot; H; \cdot \rightarrow \Xi'; \Delta'$ and \\
$\Delta_1, ..., \Delta_n$ is not empty if $A_1, ..., A_n$ is not $\cdot$.

Induction on $\Omega = A_1, ..., A_n$.

\begin{itemize}
\item $p, \Omega$ and $p \notin \Delta$

Not applicable.

\item $p, \Omega$

$\mo \Delta, \Delta_1, ..., \Delta_n, p; \Xi; p, A_1, ..., A_n; H; \cdot \rightarrow \Xi'; \Delta'$ \hfill (1) assumption \\
$\mo \Delta, \Delta_1, ..., \Delta_n; \Xi, p; A_1, ..., A_n; H; \cdot \rightarrow \Xi'; \Delta'$ \hfill (2) inversion of (1) \\
$\mz \Delta_1 ; A_1 \rightarrow \Delta_1$ ... $\mz \Delta_n ; A_n \rightarrow \Delta_n$ \hfill (3) induction on (2) \\
$\mo \Delta; \Xi, p, \Delta_1, ..., \Delta_n; \cdot ; H ; \cdot \rightarrow \Xi'; \Delta'$ \hfill (4) induction on (2) \\
$\mz p; p \rightarrow p$ \hfill (5) axiom \\
$p, \Delta_1, ..., \Delta_n$ is not empty\\

\item $A \otimes B, \Omega$

$\mo \Delta, \Delta_1, ..., \Delta_n; \Xi; A \otimes B, A_1, ..., A_{n-2}; H; \cdot \rightarrow \Xi'; \Delta'$ \hfill (1) assumption \\
$\mo \Delta, \Delta_1, ..., \Delta_n; \Xi; A, B, A_1, ..., A_{n-2}; H; \cdot \rightarrow \Xi'; \Delta'$ \hfill (2) inversion of (1) \\
$\mo \Delta; \Xi, \Delta_1, ..., \Delta_n; \cdot ; H; \cdot \rightarrow \Xi'; \Delta'$ \hfill (3) induction on (2) \\
$\mz \Delta_1 ; A \rightarrow \Delta_1$, \; $\mz \Delta_2; B \rightarrow \Delta_2$, \; ... \; $\mz \Delta_n; A_{n-2} \rightarrow \Delta_n$ \hfill (4) induction on (2) \\
$\mz \Delta_1, \Delta_2; A \otimes B \rightarrow \Delta_1, \Delta_2$ \hfill (5) rule on (4) \\
$\mz \Delta_1, \Delta_2; A \otimes B \rightarrow \Delta_1, \Delta_2$ \; ... \; $\mz \Delta_n; A_{n-2} \rightarrow \Delta_n$ \hfill (6) from (5) \\
$\Delta_1, ..., \Delta_n$ is not empty \hfill (7) from induction on (2) \\

\item $\cdot$

$\mo \Delta ; \Xi; \cdot ; H; (\cdot ; \Delta'') \rightarrow \Xi'; \Delta'$ \hfill (1) assumption \\
$n = 0$ \hfill since $\Omega = \cdot$ \\

\end{itemize}

\subsection{Derive soundness}

If $\done \Delta; \Xi; \Delta_1; \Omega; \cdot \rightarrow \Xi'; \Delta'$ then \\
$\dz \Delta; \Xi; \Delta_1; \Omega \rightarrow \Xi'; \Delta'$

By induction first on $\Omega$ and then on the size of $\Delta$.

\begin{itemize}
\item $p, \Omega$

$\done \Delta; \Xi; \Delta_1; p, \Omega; \cdot \rightarrow \Xi'; \Delta'$ \hfill (1) assumption \\
$\done \Delta; \Xi; \Delta_1, p; \Omega; \cdot \rightarrow \Xi'; \Delta'$ \hfill (2) inversion of (1) \\
$\dz \Delta; \Xi; \Delta_1, p; \Omega \rightarrow \Xi'; \Delta'$ \hfill (3) by induction on (2) \\
$\dz \Delta; \Xi; \Delta_1; p, \Omega \rightarrow \Xi'; \Delta'$ \hfill (4) rule application on (3) \\

\item $1, \Omega$

Same as before.

\item $A \otimes B, \Omega$

Same as before.

\item $\comp A \lolli B, \Omega$

$\done \Delta; \Xi; \Delta_1; \comp A \lolli B, \Omega; \cdot \rightarrow \Xi'; \Delta'$ \hfill (1) assumption \\
$\ao \Delta; A \lolli B; (\done \Delta; \Xi; \Delta_1; \comp A \lolli B, \Omega) \rightarrow \Xi'; \Delta'$ \hfill (2) inversion of (1) \\
$\mo \Delta; \cdot; A; B ; (\done \Delta; \Xi; \Delta_1; \comp A \lolli B, \Omega) \rightarrow \Xi'; \Delta'$ \hfill (3) inversion of (2) \\
Using (3) on theorem "Low level comprehension gives one match" we get two subcases:

\begin{itemize}
\item Comprehension fails:

$\cont (\done \Delta; \Xi; \Delta_1; \comp A \lolli B, \Omega); \Xi' \Delta'$ \hfill (4) from theorem \\
$\done \Delta; \Xi; \Delta_1; \Omega; \cdot \rightarrow \Xi'; \Delta'$ \hfill (5) inversion of (4) \\
$\dz \Delta; \Xi; \Delta_1; \Omega \rightarrow \Xi'; \Delta'$ \hfill (6) induction on (5) \\
$\dz \Delta; \Xi; \Delta_1; 1, \Omega \rightarrow \Xi';\Delta'$ \hfill (7) rule on (6) \\
$\dz \Delta; \Xi; \Delta_1; 1 \with (A \lolli B \otimes \comp A \lolli B), \Omega \rightarrow \Xi'; \Delta'$ \hfill (8) rule application on (7) \\
$\dz \Delta; \Xi; \Delta_1; \comp A \lolli B, \Omega \rightarrow \Xi'; \Delta'$ (9) rule application on (8) \\
\item Comprehension succeeds:
$\Delta = \Delta'', \Xi''$ \hfill (4) from theorem \\
$\mo \Delta''; \Xi''; \cdot ; B; (\done \Delta; \Xi; \Delta_1; \comp A \lolli B, \Omega) \rightarrow \Xi'; \Delta'$ \hfill (5) from theorem "Low level comprehension gives one match" \\
$\mz \Xi''; A \rightarrow \Xi''$ \hfill (6) from the same theorem \\
$\Delta''$ is smaller than $\Delta$ \hfill (7) from the same theorem \\
$\done \Delta''; \Xi''; \cdot; B; (\done \Delta; \Xi; \Delta_1; \comp A \lolli B, \Omega) \rightarrow \Xi'; \Delta'$ \hfill (8) inversion of (5) \\
$\done \Delta''; \Xi'', \Xi; \Delta_1; B, \comp A \lolli B, \Omega; \cdot \rightarrow \Xi'; \Delta'$ \hfill (9) using theorem "Comprehension head is another derivation theorem" on (8) \\
$\dz \Delta''; \Xi''; \Xi; \Delta_1; B, \comp A \lolli B, \Omega \rightarrow \Xi'; \Delta'$ \hfill (10) by i.h. on (9) because of (7) \\
$\dz \Xi'', \Delta''; \Xi'; \Delta_1; A \lolli B, \comp A \lolli B, \Omega \rightarrow \Xi'; \Delta'$ \hfill (11) using rule on (10) and (6) \\
$\dz \Xi'', \Delta''; \Xi'; \Delta_1; (A \lolli B) \otimes (\comp A \lolli B), \Omega \rightarrow \Xi'; \Delta'$ \hfill (12) using rule on (11) \\
$\dz \Xi'', \Delta''; \Xi'; \Delta_1; 1 \with ((A \lolli B) \otimes (\comp A \lolli B)), \Omega \rightarrow \Xi'; \Delta'$ \hfill (13) rule on (12) \\
$\dz \Xi'', \Delta''; \Xi'; \Delta_1; \comp A \lolli B, \Omega \rightarrow \Xi'; \Delta'$ \hfill (14) rule on (13) \\

\end{itemize}
\end{itemize}

\subsection{Apply Soundness Theorem}

If $\ao \Delta; R; (\cdot; \Delta) \rightarrow \Xi'; \Delta'$ then \\
      $\az \Delta; R \rightarrow \Xi'; \Delta'$

Case by case analysis:

\begin{itemize}
\item $R = A \lolli B$

$\ao \Delta; A \lolli B ; (\cdot ; \Delta) \rightarrow \Xi'; \Delta'$ \hfill (1) assumption \\
$\mo \Delta_1, \Delta_2; \cdot; A ; B ; (\cdot ; \Delta) \rightarrow \Xi'; \Delta'$ \hfill (2) inversion of (1) \\
$\mo \Delta_2; \Delta_1; \cdot ; B ; (\cdot ; \Delta) \rightarrow \Xi'; \Delta'$ \hfill (3) using theorem "Low level matching gives high level matching theorem" on (2) \\
$\mz \Delta_1 ; A \rightarrow \Delta_1$ \hfill (4) from same theorem on (2) \\
$\do \Delta_2; \Delta_1; \cdot ; B ; (\cdot ; \Delta) \rightarrow \Xi'; \Delta'$ \hfill (5) inversion of (3) \\
$\dz \Delta_2; \Delta_1; \cdot ; B \rightarrow \Xi'; \Delta'$ \hfill (6) derive soundness on (5) \\
$\az \Delta_1, \Delta_2; A \lolli B \rightarrow \Xi'; \Delta'$ \hfill (7) using rule on (6) and (4) \\
\end{itemize}

\subsection{Success or continuation}

If $\mo \Delta; \Xi; \Delta_1; \Omega; H; (\Phi; \Delta'') \rightarrow \Xi'; \Delta'$ then either:

\begin{itemize}
   \item $\cont \; (\Phi; \Delta''); \Xi'; \Delta'$
   \item $\mo \Delta; \Xi; \Delta_1; \Omega; H; (\cdot; \Delta'') \rightarrow \Xi'; \Delta'$
\end{itemize}

Induction on $\Omega$:

\begin{itemize}
\item $p, \Omega$ and $p \in \Omega$

$\mo \Delta, p; \Xi; p, \Omega; H; (\Phi; \Delta'') \rightarrow \Xi'; \Delta'$ \hfill (1) assumption\\
$\mo \Delta; \Xi, p; \Omega; H; (\Phi; \Delta'') \rightarrow \Xi'; \Delta'$ \hfill (2) inversion of (1)\\
$\cont \; (\Phi; \Delta'') ; \Xi'; \Delta'$ or $\mo \Delta; \Xi, p; \Omega; H; (\cdot; \Delta'') \rightarrow \Xi'; \Delta'$ \hfill (3) induction of (2) \\
$\cont \; (\Phi; \Delta'') ; \Xi'; \Delta'$ or $\mo \Delta, p; \Xi; p, \Omega; H; (\cdot; \Delta'') \rightarrow \Xi'; \Delta'$ \hfill (4) rule application on (3) \\

\item $p, \Omega$ and $p \notin \Delta$

$\mo \Delta; \Xi; p, \Omega; H; (\Phi; \Delta'') \rightarrow \Xi'; \Delta'$ \hfill (1) assumption \\
$\cont \; (\Phi; \Delta''); \Xi'; \Delta'$ \hfill (2) inversion of (1) \\

\item $A \otimes B, \Omega$

$\mo \Delta; \Xi; A \otimes B, \Omega; H; (\Phi; \Delta'') \rightarrow \Xi'; \Delta'$ \hfill (1) assumption \\
$\mo \Delta; \Xi; A, B, \Omega; H; (\Phi; \Delta'') \rightarrow \Xi'; \Delta'$ \hfill (2) inversion of (1) \\
$\cont \; (\Phi; \Delta''); \Xi'; \Delta'$ or $\mo \Delta; \Xi; A, B, \Omega; H; (\cdot; \Delta'') \rightarrow \Xi'; \Delta'$ \hfill (3) i.h. on (2) \\
$\cont \; (\Phi; \Delta''); \Xi'; \Delta'$ or $\mo \Delta; \Xi; A \otimes B, \Omega; H; (\cdot; \Delta'') \rightarrow \Xi'; \Delta'$ \hfill (4) rule on (3) \\

\item $\cdot$

$\mo \Delta; \Xi; \cdot; H; (\Phi; \Delta'') \rightarrow \Xi'; \Delta'$ \hfill (1) assumption \\
$\done \Delta; \Xi; \cdot; H; \cdot \rightarrow \Xi'; \Delta'$ \hfill (2) inversion of (1) \\
$\mo \Delta; \Xi; \cdot; H; (\cdot; \Delta'') \rightarrow \Xi'; \Delta'$ \hfill (3) rule application on (2) \\
\end{itemize}

\subsection{One Rule Theorem}

If $\doo \Delta; \Phi \rightarrow \Xi'; \Delta'$ then $\exists R \in \Phi. \doo \Delta; R \rightarrow \Xi'; \Delta'$.

Induction on the size of $\Phi$.

\begin{itemize}
\item $\Phi = \cdot$

Not applicable.

\item $\Phi = R', \Phi'$

$\doo \Delta; R', \Phi' \rightarrow \Xi' \Delta'$ \hfill (1) assumption \\
$\ao \Delta; R'; (\Phi'; \Delta) \rightarrow \Xi'; \Delta'$ \hfill (2) inversion of (1) \\
$\mo \Delta; \cdot; A; B; (\Phi'; \Delta) \rightarrow \Xi'; \Delta'$ \hfill (3) inversion of (2) where $R' = A \lolli B$\\

From theorem "Success or continuation" we have two cases:

   \begin{itemize}
   \item Match Success \\
   $\mo \Delta; \cdot; A; B; (\cdot; \Delta) \rightarrow \Xi'; \Delta'$ \hfill (4) from theorem \\
   $\ao \Delta; A \lolli B; (\cdot; \Delta) \rightarrow \Xi'; \Delta'$ \hfill (5) rule application on (4) \\
   $\doo \Delta; A \lolli B \rightarrow \Xi'; \Delta'$ \hfill (6) rule application on (5) \\
   $\doo \Delta; R \rightarrow \Xi'; \Delta'$ \hfill (7) rewrite of (6) \\

   \item Continuation \\
   $\cont (\Phi'; \Delta); \Xi'; \Delta'$ \hfill (4) from theorem \\
   $\doo \Delta; \Phi' \rightarrow \Xi'; \Delta'$ \hfill (5) inversion of (4) \\
   $\exists R \in \Phi'. \doo \Delta; R \rightarrow \Xi'; \Delta'$ \hfill (6) i.h. on (5) \\
   $\exists R \in \Phi.$ \hfill (7) from (6) \\
   \end{itemize}

\end{itemize}