
\subsection{Low Level System}

For this system, we include only linear facts but we use a continuation stack to match facts.

\subsubsection{Match}

\[
\infer[ok]
{\mo \Delta, p_1, \Delta'' ; \Xi; p, \Omega; H; C; R \rightarrow \Xi'; \Delta'}
{\mo \Delta, \Delta''; \Xi, p_1; \Omega; H; (\Delta, p_1; \Delta''; p, \Omega; H; \Xi), C; R \rightarrow \Xi'; \Delta'}
\tab
\infer[fail]
{\mo \Delta; \Xi; p, \Omega; H; C; R \rightarrow \Xi'; \Delta'}
{p \notin \Delta & \cont C ; R; \Xi'; \Delta'}
\]

\[
\infer[match \; \otimes]
{\mo \Delta; \Xi; A \otimes B, \Omega ; H ; C; R \rightarrow \Xi'; \Delta'}
{\mo \Delta; \Xi; A, B, \Omega; H; C; R \rightarrow \Xi';\Delta'}
\]

\[
\infer[end]
{\mo \Delta; \Xi; \cdot ; H; C; R \rightarrow \Xi'; \Delta'}
{\done \Delta; \Xi; \cdot ; H; \cdot \rightarrow \Xi'; \Delta'}
\]

\subsubsection{Derive}

\[
\infer[derive \; p]
{\done \Delta; \Xi; \Delta_1; p, \Omega; C \rightarrow \Xi'; \Delta'}
{\done \Delta; \Xi; p, \Delta_1; \Omega; C \rightarrow \Xi'; \Delta'}
\tab
\infer[derive \; 1]
{\done \Delta; \Xi; \Delta_1; 1, \Omega; C \rightarrow \Xi';\Delta'}
{\done \Delta; \Xi; \Delta_1; \Omega; C \rightarrow \Xi'; \Delta'}
\]

\[
\infer[derive \; \otimes]
{\done \Delta; \Xi; \Delta_1; A \otimes B, \Omega; C \rightarrow \Xi'; \Delta'}
{\done \Delta; \Xi; \Delta_1; A, B, \Omega; C \rightarrow \Xi';\Delta'}
\]

\[
\infer[derive \; end]
{\done \Delta; \Xi; \Delta_1; \cdot \rightarrow \Xi; \Delta_1}
{}
\]

\subsubsection{Continuation}

\[
\infer[next \; rule]
{\cont \cdot; (\Phi; \Delta); \Xi'; \Delta'}
{\doo \Delta; \Phi \rightarrow \Xi'; \Delta'}
\]

\[
\infer[cont \; next]
{\cont (\Delta; p_1, \Delta''; p, \Omega; H; \Xi), C; R; \Xi'; \Delta'}
{\mo \Delta, \Delta''; \Xi, p_1; \Omega; H; (\Delta, p_1; \Delta''; p, \Omega; H; \Xi), C; R \rightarrow \Xi'; \Delta'}
\]

\[
\infer[cont \; no \; more]
{\cont (\Delta; \cdot; p, \Omega; H; \Xi), C; R; \Xi'; \Delta'}
{\cont C; R; \Xi'; \Delta'}
\]

\subsubsection{Apply}

\[
\infer[start \; matching]
{\ao \Delta; A \lolli B; R \rightarrow \Xi'; \Delta'}
{\mo \Delta; \cdot; A; B; \cdot; R \rightarrow \Xi'; \Delta'}
\]

\[
\infer[do \; rule]
{\doo \Delta; R, \Phi \rightarrow \Xi'; \Delta'}
{\ao \Delta; R; (\Phi; \Delta) \rightarrow \Xi';\Delta'}
\]

\input{high-level-simple}

\subsection{Theorems}

\subsubsection{Match soundness theorem}

If $\mo \Delta, \Delta_1, ..., \Delta_n; \Xi; \Omega_1, ..., \Omega_n; H; C; R \rightarrow \Xi'; \Delta'$ then either:\\
1. \hspace{1cm} $\cont \cdot; R; \Xi'; \Delta'$ or \\
2. \hspace{1cm} $\mo \Delta; \Xi, \Delta_1, ..., \Delta_n; \cdot; H; C''; R \rightarrow \Xi'; \Delta'$ and $\mz \Delta_1; \Omega_1 \rightarrow \Delta_1$ ... $\mz \Delta_n; \Omega_n \rightarrow \Delta_n$ or \\
3. \hspace{1cm} $\exists f = (\Delta_a; \Delta_b; \Omega_1, ..., \Omega_n; H; \Xi_a) \in C$ such that:\\
3.1 \hspace{2cm} $\Delta_a, \Delta_b = \Delta_c, \Delta_1, ..., \Delta_n$ and \\
3.2 \hspace{2cm} $\mo \Delta_c; \Xi_a, \Delta_1, ..., \Delta_n; \cdot; H; C''; R \rightarrow \Xi'; \Delta'$ and \\
3.3 \hspace{2cm} $\mz \Delta_1; \Omega_1 \rightarrow \Delta_1$ ... $\mz \Delta_n; \Omega_n \rightarrow \Delta_n$.\\

If $\cont C; R; \Xi'; \Delta'$ then either:\\
1. \hspace{1cm} $\cont \cdot; R; \Xi'; \Delta'$ or \\
2. \hspace{1cm} $\exists f = (\Delta_a; \Delta_b; \Omega_1, ..., \Omega_n; H; \Xi_a) \in C$ such that:\\
2.1 \hspace{2cm} $\Delta_a, \Delta_b = \Delta_c, \Delta_1, ..., \Delta_n$ and \\
2.2 \hspace{2cm} $\mo \Delta_c; \Xi_a, \Delta_1, ..., \Delta_n; \cdot; H; C''; R \rightarrow \Xi'; \Delta'$ and \\
2.3 \hspace{2cm} $\mz \Delta_1; \Omega_1 \rightarrow \Delta_1$ ... $\mz \Delta_n; \Omega_n \rightarrow \Delta_n$.\\

Proof by mutual induction. In $\mo$ on the size of $\Omega$ and on $\cont$ on the size of $C$ and $\Delta''$.

\begin{itemize}
   \item $ok$
   
   By induction.
   
   \item $fail$
   
   $\mo \Delta; \Xi; p, \Omega; H; C; R \rightarrow \Xi'; \Delta'$ \hfill (1) assumption \\
   $\cont C; R; \Xi'; \Delta'$ \hfill (2) inversion of (1) \\
   Apply i.h. on (2) to get $\cont \cdot; R; \Xi'; \Delta'$ or the $\exists f.$.
   
   \item $match \; \otimes$
   
   By induction.
   
   \item $end$
   
   $\mz \Delta; \Xi; \cdot; H; C; R \rightarrow \Xi'; \Delta'$ \hfill (1) assumption.\\
   
   \item $next \; rule$
   
   $\cont \cdot; (\Phi; \Delta); \Xi'; \Delta'$ \hfill (1) assumption \\
   
   \item $cont \; next$ -- some doubts about this one.
   
   $\cont (\Delta; p_1, \Delta''; p, \Omega; H; \Xi), C; R; \Xi'; \Delta'$ \hfill (1) assumption \\
   $\mo \Delta, \Delta''; \Xi, p_1;  \Omega; H; (\Delta, p_1; \Delta''; p, \Omega; H; \Xi), C; R \rightarrow \Xi'; \Delta'$ \hfill (2) inversion of (1)\\
   Induction on (2):
   
   \begin{itemize}
      \item $\cont \cdot; R; \Xi'; \Delta'$
      
      \item $\mo \Delta_a; \Xi, p_1, \Delta_1, ..., \Delta_n; \cdot; H; C''; R \rightarrow \Xi'; \Delta'$ 
      
      where $\Delta_a, \Delta_1, ..., \Delta_n = \Delta, \Delta'$ \\
      
      $\exists f = (\Delta; p_1; \Delta''; p, \Omega; H; \Xi)$
      
      \item $\exists f \in (\Delta, p_1; \Delta''; p, \Omega; H; \Xi), C$
      
      $f$ can be $(\Delta, p_1; \Delta''; p, \Omega; H; \Xi)$ (which is contained in the original $\cont$)\\
      or $f \in C$\\
      
   \end{itemize}
   
   \item $cont \; no \; more$
   
   $\cont (\Delta; \cdot; p, \Omega; H; \Xi), C; R; \Xi'; \Delta'$ \hfill (1) assumption \\
   $\cont C; R; \Xi'; \Delta'$ \hfill (2) inversion of (1) \\
   
   By induction:
   
   \begin{itemize}
      \item $\cont \cdot; R; \Xi'; \Delta'$
      
      \item $\exists f \in C$
      
      Then $\exists f \in (\Delta; \cdot; p, \Omega; H; \Xi), C$ \\
   \end{itemize}
   
\end{itemize}

\subsection{Match Soundness Lemma}

If $\mo \Delta, \Delta''; \cdot; \Omega; H; \cdot; R \rightarrow \Xi'; \Delta'$ then either:\\
1. \hspace{1cm} $\cont \cdot; R; \Xi'; \Delta'$ or \\
2. \hspace{1cm} $\mo \Delta; \Delta''; \cdot; H; C'; R \rightarrow \Xi'; \Delta'$ and\\
2.1 \hspace{2cm} $\mz \Delta''; \Omega \rightarrow \Delta''$\\

Proof: By direct use of the match soundness theorem.

\subsection{Derive Soundness Theorem}

If $\done \Delta; \Xi; \Delta_1; \Omega; C \rightarrow \Xi'; \Delta'$ then $\dz \Delta; \Xi; \Delta_1; \Omega \rightarrow \Xi'; \Delta'$.

By simple induction on $\Omega$.

\begin{itemize}
   \item $derive \; p$
   
   By induction.
   
   \item $derive \; 1$
   
   By induction.
   
   \item $derive \; \otimes$
   
   By induction.
   
   \item $derive \; end$
   
   Use axioms.
   
\end{itemize}