

\input{high-level}

\subsection{Low Level System}

We extend the previous system with comprehensions.

\subsubsection{Match}

\[
\infer[\mo ok]
{\mo \Delta, p_1, \Delta'' ; \Xi; p, \Omega; H; C; R \rightarrow \Xi'; \Delta'}
{\mo \Delta, \Delta''; \Xi, p_1; \Omega; H; (\Delta, p_1; \Delta''; p, \Omega; H; \Xi), C; R \rightarrow \Xi'; \Delta'}
\tab
\infer[\mo fail]
{\mo \Delta; \Xi; p, \Omega; H; C; R \rightarrow \Xi'; \Delta'}
{p \notin \Delta & \cont C ; R; \Xi'; \Delta'}
\]

\[
\infer[\mo \otimes]
{\mo \Delta; \Xi; A \otimes B, \Omega ; H ; C; R \rightarrow \Xi'; \Delta'}
{\mo \Delta; \Xi; A, B, \Omega; H; C; R \rightarrow \Xi';\Delta'}
\]

\[
\infer[\mo end]
{\mo \Delta; \Xi; \cdot ; H; C; R \rightarrow \Xi'; \Delta'}
{\done \Delta; \Xi; \cdot ; H; \cdot \rightarrow \Xi'; \Delta'}
\]

\subsubsection{Derive}

\newcommand{\mc}[0]{\m{mc} \; }
\newcommand{\dall}[0]{\m{dall} \; }

\[
\infer[\done p]
{\done \Delta; \Xi; \Delta_1; p, \Omega; C \rightarrow \Xi'; \Delta'}
{\done \Delta; \Xi; p, \Delta_1; \Omega; C \rightarrow \Xi'; \Delta'}
\tab
\infer[\done 1]
{\done \Delta; \Xi; \Delta_1; 1, \Omega; C \rightarrow \Xi';\Delta'}
{\done \Delta; \Xi; \Delta_1; \Omega; C \rightarrow \Xi'; \Delta'}
\]

\[
\infer[\done \otimes]
{\done \Delta; \Xi; \Delta_1; A \otimes B, \Omega; C \rightarrow \Xi'; \Delta'}
{\done \Delta; \Xi; \Delta_1; A, B, \Omega; C \rightarrow \Xi';\Delta'}
\]

\[
\infer[\done end]
{\done \Delta; \Xi; \Delta_1; \cdot \rightarrow \Xi; \Delta_1}
{}
\]

\[
\infer[\done comp]
{\done \Delta ; \Xi; \Delta_1; \comp A \lolli B, \Omega \rightarrow \Xi';\Delta'}
{\mc \Delta; \Xi; \Delta_1; \cdot; A ; B ; \cdot; \comp A \lolli B; \Omega; \Delta \rightarrow \Xi';\Delta'}
\]

\subsubsection{Continuation}

\[
\infer[\cont next \; rule]
{\cont \cdot; (\Phi; \Delta); \Xi'; \Delta'}
{\doo \Delta; \Phi \rightarrow \Xi'; \Delta'}
\]

\[
\infer[\cont next]
{\cont (\Delta; p_1, \Delta''; p, \Omega; H; \Xi), C; R; \Xi'; \Delta'}
{\mo \Delta, \Delta''; \Xi, p_1; \Omega; H; (\Delta, p_1; \Delta''; p, \Omega; H; \Xi), C; R \rightarrow \Xi'; \Delta'}
\]

\[
\infer[\cont no \; more]
{\cont (\Delta; \cdot; p, \Omega; H; \Xi), C; R; \Xi'; \Delta'}
{\cont C; R; \Xi'; \Delta'}
\]

\subsubsection{Match Comprehension}

\[
\infer[\mc p \; ok \; first]
{\mc \Delta, p_1, \Delta''; \Xi_N; \Delta_{N1}; \Xi; p, \Omega; \cdot; AB; \Omega_N; \Delta_N \rightarrow \Xi'; \Delta'}
{\mc \Delta, \Delta''; \Xi_N; \Delta_{N1}; \Xi, p_1; \Omega; (\Delta, p_1; \Delta''; \Xi; p; \Omega; \cdot); AB; \Omega_N; \Delta_N \rightarrow \Xi'; \Delta'}
\]

\[
\infer[\mc p \; ok \; other]
{\mc \Delta, p_1, \Delta''; \Xi_N; \Delta_{N1}; \Xi; p, \Omega; C_1, C; AB; \Omega_N; \Delta_N \rightarrow \Xi'; \Delta'}
{\mc \Delta, \Delta''; \Xi_N; \Delta_{N1}; \Xi, p_1; \Omega; (\Delta, p_1; \Delta''; \Xi; p; \Omega; q, \Lambda), C_1, C; AB; \Omega_N; \Delta_N \rightarrow \Xi'; \Delta' & C1 = (\Delta_{old}; \Delta'_{old}; \Xi_{old}; q; \Omega_{old}; \Lambda)}
\]


\[
\infer[\mc p \; fail]
{\mc \Delta; \Xi_N; \Delta_{N1}; \Xi; p, \Omega; C; \comp A \lolli B; \Omega_N; \Delta_N \rightarrow \Xi'; \Delta'}
{\contc \Delta_N; \Xi_N; \Delta_{N1}; C; \comp A \lolli B; \Omega_N \rightarrow \Xi'; \Delta'}
\]

\[
\infer[\mc \otimes]
{\mc \Delta; \Xi_N; \Delta_{N1}; \Xi; X \otimes Y, \Omega; C; \comp A \lolli B; \Omega_N; \Delta_N \rightarrow \Xi'; \Delta'}
{\mc \Delta; \Xi_N; \Delta_{N1}; \Xi; X, Y, \Omega; C; \comp A \lolli B; \Omega_N; \Delta_N \rightarrow \Xi'; \Delta'}
\]

\[
\infer[\mc end]
{\mc \Delta; \Xi_N; \Delta_{N1}; \Xi; \cdot; C; \comp A \lolli B; \Omega_N; \Delta_N \rightarrow \Xi'; \Delta'}
{\dall \Xi_N; \Delta_{N1}; \Xi; C; \comp A \lolli B; \Omega_N; \Delta_N \rightarrow \Xi'; \Delta'}
\]

\[
\infer[\dall end]
{\dall \Xi_N; \Delta_{N1}; \Xi; (\Delta_x; \Delta''; \cdot; p, \Omega; \cdot); \comp A \lolli B; \Omega_N; \Delta_N \rightarrow \Xi'; \Delta'}
{\dc \Xi_N, \Xi; \Delta_{N1}; (\Delta_x - \Xi; \Delta'' - \Xi; \cdot; p; \Omega; \cdot) ; \comp A \lolli B; \Omega_N; (\Delta_N - \Xi) \rightarrow \Xi'; \Delta'}
\]

\[
\infer[\dall more]
{\dall \Xi_N; \Delta_{N1}; \Xi; \_, X, C; \comp A \lolli B; \Omega_N; \Delta_N \rightarrow \Xi'; \Delta'}
{\dall \Xi_N; \Delta_{N1}; \Xi; X, C; \comp A \lolli B; \Omega_N; \Delta_N \rightarrow \Xi'; \Delta'}
\]

\[
\infer[\dc p]
{\dc \Xi; \Delta_1; p, \Omega; C; \comp A \lolli B; \Omega_N; \Delta_N \rightarrow \Xi'; \Delta'}
{\dc \Xi; \Delta_1, p; \Omega; C; \comp A \lolli B; \Omega_N; \Delta_N \rightarrow \Xi'; \Delta'}
\]

\[
\infer[\dc \otimes]
{\dc \Xi; \Delta_1; A \otimes B, \Omega; C; \comp A \lolli B; \Omega_N; \Delta_N \rightarrow \Xi'; \Delta'}
{\dc \Xi; \Delta_1; A, B, \Omega; C; \comp A \lolli B; \Omega_N; \Delta_N \rightarrow \Xi'; \Delta'}
\]

\[
\infer[\dc end]
{\dc \Xi; \Delta_1; \cdot; C; \comp A \lolli B; \Omega_N; \Delta_N \rightarrow \Xi'; \Delta'}
{\contc \Delta_N; \Xi; \Delta_1; C; \comp A \lolli B; \Omega_N \rightarrow \Xi'; \Delta'}
\]

\subsubsection{Match Comprehension Continuation}

\[
\infer[\contc end]
{\contc \Delta_N; \Xi_N; \Delta_{N1}; \cdot; \comp A \lolli B; \Omega \rightarrow \Xi'; \Delta'}
{\done \Delta_N; \Xi_N; \Delta_{N1}; \Omega \rightarrow \Xi'; \Delta'}
\]

\[
\infer[\contc next]
{\contc \Delta_N; \Xi_N; \Delta_{N1}; (\Delta; p_1, \Delta''; \Xi; p; \Omega; \Lambda), C; AB; \Omega_N \rightarrow \Xi'; \Delta'}
{\mc \Delta; \Xi_N; \Delta_{N1}; \Xi; \Omega; (\Delta, p_1; \Delta''; \Xi; p; \Omega; \Lambda), C; AB; \Omega_N; \Delta_N \rightarrow \Xi'; \Delta'}
\]

\[
\infer[\contc next \; empty]
{\contc \Delta_N; \Xi_N; \Delta_{N1}; (\Delta; \cdot; \Xi; p; \Omega; \Lambda), C; AB; \Omega_N \rightarrow \Xi'; \Delta'}
{\contc \Delta_N; \Xi_N; \Delta_{N1}; C; AB; \Omega_N \rightarrow \Xi'; \Delta'}
\]

\subsubsection{Apply}

\[
\infer[\ao start \; matching]
{\ao \Delta; A \lolli B; R \rightarrow \Xi'; \Delta'}
{\mo \Delta; \cdot; A; B; \cdot; R \rightarrow \Xi'; \Delta'}
\]

\[
\infer[\doo rule]
{\doo \Delta; R, \Phi \rightarrow \Xi'; \Delta'}
{\ao \Delta; R; (\Phi; \Delta) \rightarrow \Xi';\Delta'}
\]

\subsection{Flat Equivalence}

\newcommand{\flatten}[0]{\m{flatten} \;}

\newcommand{\feq}[2]{#1 \equiv #2}

\[
\infer[\equiv p]
{\feq{p, A}{p, B}}
{\feq{A}{B}}
\]

\[
\infer[\equiv 1 \; left]
{\feq{1, A}{B}}
{\feq{A}{B}}
\tab
\infer[\equiv 1 \; right]
{\feq{A}{1, B}}
{\feq{A}{B}}
\]

\[
\infer[\equiv \cdot]
{\feq{\cdot}{\cdot}}
{}
\]

\[
\infer[\equiv left]
{\feq{A \otimes B, C}{D}}
{\feq{A, B, C}{D}}
\tab
\infer[\equiv right]
{\feq{A}{B \otimes C, D}}
{\feq{A}{B, C, D}}
\]

\subsubsection{Equivalence commutativity}

If $\feq{A}{B}$ then $\feq{B}{A}$.

\begin{proof}
   By induction on the structure of the assumption.
   
   \begin{itemize}
      \item $p$
      
      $\feq{p, A}{p, B}$ \hfill (1) assumption \\
      $\feq{A}{B}$ \hfill (2) inversion of (1) \\
      $\feq{B}{A}$ \hfill (3) i.h. on (2) \\
      $\feq{p, B}{p, A}$ \hfill (4) rule on (3) \\
      
      \item $1 \; left$
      
      $\feq{1, A}{B}$ \hfill (1) assumption \\
      $\feq{A}{B}$ \hfill (2) assumption \\
      $\feq{B}{A}$ \hfill (3) i.h. on (2) \\
      $\feq{B}{1, A}$ \hfill (4) apply right rule on (3) \\
      
      \item $1 \; right$
      
      Same thing as before.
      
      \item $\cdot$
      
      Immediate.
      
      \item $left$
      
      $\feq{A \otimes B, C}{D}$ \hfill (1) assumption \\
      $\feq{A, B, C}{D}$ \hfill (2) inversion of (1) \\
      $\feq{D}{A, B, C}$ \hfill (3) i.h. on (2) \\
      $\feq{D}{A \otimes B, C}$ \hfill (4) right rule on (3) \\
      
      \item $right$
      
      Same thing as the last case.
   \end{itemize}
\end{proof}

\subsubsection{Match Equivalence Theorem}

If $\feq{A_1, ..., A_n}{B_1, ..., B_m}$ and $\mz \Delta; A_1 \otimes ... \otimes A_n \rightarrow \Delta$ then $\mz \Delta; B_1 \otimes ... \otimes B_m \rightarrow \Delta$.

\begin{proof}
   By induction on the structure of the assumption.
   
   \begin{itemize}
      \item $p$
      
      $\feq{p, A}{p, B}$ \hfill (1) assumption \\
      $\feq{A}{B}$ \hfill (2) assumption \\
      $\mz p; p \rightarrow p$ \hfill (3) axiom \\
      $\mz p, \Delta; p \otimes A \rightarrow p, \Delta$ \hfill (4) assumption \\
      $\mz \Delta; A \rightarrow \Delta$ \hfill (5) inversion of (4) \\
      $\mz \Delta; B \rightarrow \Delta$ \hfill (6) i.h. on (5) and (2) \\
      $\mz p, \Delta; p \otimes B \rightarrow p, \Delta$ \hfill (7) rule application on (6) and (3) \\
      
      \item $1 \; left$
      
      $\feq{1, A}{B}$ \hfill (1) assumption \\
      $\feq{A}{B}$ \hfill (2) assumption \\
      $\mz \Delta; 1 \otimes A \rightarrow \Delta$ \hfill (3) assumption \\
      $\mz \Delta; A \rightarrow \Delta$ \hfill (4) inversion of (4) \\
      $\mz \cdot; 1 \rightarrow \cdot$ \hfill (5) axiom \\
      $\mz \Delta; B \rightarrow \Delta$ \hfill (6) i.h. on (2) and (4) \\
      $\mz \Delta; 1 \otimes B \rightarrow \Delta$ \hfill (7) rule application on (6) and (5) \\
      
      \item $1 \; right$
      
      Same thing as before.
      
      \item $\cdot$
      
      Immediate since $\mz$ fails.
      
      \item $\otimes \; left$
      
      $\feq{A \otimes B, C}{D}$ \hfill (1) assumption \\
      $\feq{A, B, C}{D}$ \hfill (2) inversion of (1) \\
      $\mz \Delta_1, \Delta_2, \Delta_3; (A \otimes B) \otimes C \rightarrow \Delta_1, \Delta_2, \Delta_3$ \hfill (3) assumption \\
      $\mz \Delta_1, \Delta_2; A \otimes B \rightarrow \Delta_1, \Delta_2$ \hfill (4) inversion of (3) \\
      $\mz \Delta_3; C \rightarrow \Delta_3$ \hfill (5) inversion of (3) \\
      $\mz \Delta_1; A \rightarrow \Delta_1$ and $\mz \Delta_2; B \rightarrow \Delta_2$ \hfill (6) inversion of (4) \\
      $\mz \Delta_1, \Delta_2, \Delta_3; A \otimes B \otimes C \rightarrow \Delta_1, \Delta_2, \Delta_3$ \hfill (7) apply (5) with (6) \\
      $\mz \Delta_1, \Delta_2, \Delta_3; D \rightarrow \Delta_1, \Delta_2, \Delta_3$ \hfill (8) i.h. on (7) and (2)\\
      
      \item $\otimes \; right$
      
      Apply equivalence commutativity theorem and follow the previous case.
   \end{itemize}
\end{proof}

\subsection{Continuation frame and stack properties}

\subsubsection{Flat Property}

Given a frame $f = (\Delta; \Delta''; \Xi; p; \Omega_1, ..., \Omega_n; \Lambda_1, ..., \Lambda_m)$ and a body term $A$, we say that $f$ follows the flat property if $\feq{p, \Omega_1, ..., \Omega_n, \Lambda_1, ..., \Lambda_m}{A}$.

\subsubsection{Flat well-formed}

A continuation stack $C$ is "flat" well-formed if every frame follows the flat property.

\subsubsection{Resource Invariant}

A frame $f = (\Delta'; \Delta''; \Xi; p; \Omega_1, ..., \Omega_n; \Lambda_1, ..., \Lambda_m)$ is resource invariant in relation to a $\Delta$ context if $\Delta', \Delta'', \Xi = \Delta$.

A continuation stack $C$ is resource invariant in relation to a $\Delta$ context if $\forall f \in C. f$ is resource invariant in relation to $\Delta$.

\subsection{Theorems}

\subsubsection{Body Match Soundness}

If $\mo \Delta, \Delta_1, ..., \Delta_n; \Xi; \Omega_1, ..., \Omega_n; H; C; R \rightarrow \Xi'; \Delta'$ then either:\\
1. \hspace{1cm} $\cont \cdot; R; \Xi'; \Delta'$ or \\
2. \hspace{1cm} $\mo \Delta; \Xi, \Delta_1, ..., \Delta_n; \cdot; H; C''; R \rightarrow \Xi'; \Delta'$ and $\mz \Delta_1; \Omega_1 \rightarrow \Delta_1$ ... $\mz \Delta_n; \Omega_n \rightarrow \Delta_n$ or \\
3. \hspace{1cm} $\exists f = (\Delta_a; \Delta_b; \Omega_1, ..., \Omega_n; H; \Xi_a) \in C$ such that:\\
3.1 \hspace{2cm} $\Delta_a, \Delta_b = \Delta_c, \Delta_1, ..., \Delta_n$ and \\
3.2 \hspace{2cm} $\mo \Delta_c; \Xi_a, \Delta_1, ..., \Delta_n; \cdot; H; C''; R \rightarrow \Xi'; \Delta'$ and \\
3.3 \hspace{2cm} $\mz \Delta_1; \Omega_1 \rightarrow \Delta_1$ ... $\mz \Delta_n; \Omega_n \rightarrow \Delta_n$.\\

If $\cont C; R; \Xi'; \Delta'$ then either:\\
1. \hspace{1cm} $\cont \cdot; R; \Xi'; \Delta'$ or \\
2. \hspace{1cm} $\exists f = (\Delta_a; \Delta_b; \Omega_1, ..., \Omega_n; H; \Xi_a) \in C$ such that:\\
2.1 \hspace{2cm} $\Delta_a, \Delta_b = \Delta_c, \Delta_1, ..., \Delta_n$ and \\
2.2 \hspace{2cm} $\mo \Delta_c; \Xi_a, \Delta_1, ..., \Delta_n; \cdot; H; C''; R \rightarrow \Xi'; \Delta'$ and \\
2.3 \hspace{2cm} $\mz \Delta_1; \Omega_1 \rightarrow \Delta_1$ ... $\mz \Delta_n; \Omega_n \rightarrow \Delta_n$.\\

\begin{proof}
Proved in Section~\ref{thm:match_soundness_basic}.
\end{proof}

\subsubsection{Comprehension soundness theorem}

\begin{itemize}
   \item Match sub-theorem

If $\mc \Delta, \Delta_1, ..., \Delta_n; \Xi_N; \Delta_{N1}; \Xi; \Omega_1, ..., \Omega_n; C; \comp A \lolli B; \Omega_N; \Delta_N \rightarrow \Xi'; \Delta'$  and $C$ is flat well-formed in respect to $A$ and $C$ is resource invariant in relation to $\Delta, \Delta_1, ..., \Delta_n, \Xi$ and $\Delta, \Delta_1, ..., \Delta_n, \Xi = \Delta_N$:\\

The matching will fail (1), succeed without using any continuation frame in $C$ (2) or it needs to backtrack to a frame in $C$ (3):\\
1. \hspace{1cm} $\done \Delta_N; \Xi_N; \Delta_{N1}; \Omega_N \rightarrow \Xi'; \Delta'$; \\
2. \hspace{1cm} $\mc \Delta; \Xi_N; \Delta_{N1}; \Xi, \Delta_1, ..., \Delta_n; \cdot; C', C; \comp A \lolli B; \Omega_N; \Delta_N \rightarrow \Xi'; \Delta'$ and\\
2.1 \hspace{2cm} $\mz \Delta_1; \Omega_1 \rightarrow \Delta_1$ ... $\mz \Delta_n; \Omega_n \rightarrow \Delta_n$\\
2.2 \hspace{2cm} $C'$ is flat well-formed in relation to $A$. \\
2.3 \hspace{2cm} $C'$ is resource invariant in relation to $\Delta, \Delta_1, ..., \Delta_n, \Xi$.\\
3. \hspace{1cm} $C = C_1, f, C_2$ and $f = (\Delta_a; \Delta_{b_1}, \Delta_{b_2}; \Xi_1, ..., \Xi_m; p; \Omega'_1, ..., \Omega'_k; \Lambda_1, ..., \Lambda_m)$ turns into $f' = (\Delta_a, \Delta_{b_1}; \Delta_{b_2}; \Xi_1, ..., \Xi_m; p; \Omega'_1, ..., \Omega'_k; \Lambda_1, ..., \Lambda_m)$ and\\
3.1 \hspace{2cm} $\Delta_a, \Delta_{b1}, \Delta_{b2} = \Delta_c, p, \Delta_1, ..., \Delta_k$ \\
3.2 \hspace{2cm} $\mc \Delta_c; \Xi_N; \Delta_{N1}; \Xi_1, ..., \Xi_m, \Delta_1, ..., \Delta_k; \cdot; C'_1, f', C_2; \comp A \lolli B; \Omega_N; \Delta_N \rightarrow \Xi'; \Delta'$.\\
3.3 \hspace{2cm} $C'_1, f'$ are flat well-formed in relation to $A$. \\
3.4 \hspace{2cm} $C'_1, f'$ are resource invariant in relation to $\Delta, \Delta_1, ..., \Delta_n, \Xi$ \\
3.5 \hspace{2cm} $\mz p; p \rightarrow p$, $\mz \Delta_1; \Omega'_1 \rightarrow \Delta_1$ ... $\mz \Delta_k; \Omega'_k \rightarrow \Delta_k$ and $\mz \Xi_1; \Lambda_1 \rightarrow \Xi_1$ ... $\mz \Xi_m; \Lambda_m \rightarrow \Xi_m$\\

We assume the following "context constraint" to be true:\\

1. If $C = \cdot$ then $\feq{A}{\Omega_1, ..., \Omega_n}$.\\
2. If $C = (\Delta_a; \Delta_b; \Xi; p; \Omega; \Lambda_1, ..., \Lambda_m), C'$ then $\feq{A}{p, \Omega_1, ..., \Omega_n, \Lambda_1, ..., \Lambda_m}$ and $\feq{\Omega_1, ..., \Omega_n}{\Omega}$.

\item Continuation sub-theorem

If $\contc \Delta_N; \Xi_N; \Delta_{N1}; C; \comp A \lolli B; \Omega_N \rightarrow \Xi'; \Delta'$ and $C$ is flat well-formed in respect to $A$ and resource invariant in relation to $\Delta_N$: \\
1. \hspace{1cm} $\done \Delta_N; \Xi_N; \Delta_{N1}; \Omega_N \rightarrow \Xi'; \Delta'$ or \\
2. \hspace{1cm} $C = C_1, f, C_2$ and $f = (\Delta_a; \Delta_{b_1}, \Delta_{b_2}; \Xi_1, ..., \Xi_m; p; \Omega'_1, ..., \Omega'_k; \Lambda_1, ..., \Lambda_m)$ turns into $f' = (\Delta_a, \Delta_{b_1}; \Delta_{b_2}; \Xi_1, ..., \Xi_m; p; \Omega'_1, ..., \Omega'_k; \Lambda_1, ..., \Lambda_m)$ and\\
2.1 \hspace{2cm} $\Delta_a, \Delta_{b1}, \Delta_{b2} = \Delta_c, p, \Delta_1, ..., \Delta_k$. \\
2.2 \hspace{2cm} $\mc \Delta_c; \Xi_N; \Delta_{N1}; \Xi_1, ..., \Xi_m, \Delta_1, ..., \Delta_k; \cdot; C'_1, f', C_2; \comp A \lolli B; \Omega_N; \Delta_N \rightarrow \Xi'; \Delta'$. \\
2.3 \hspace{2cm} $C'_1, f'$ are flat well-formed in relation to $A$. \\
2.4 \hspace{2cm} $C'_1, f'$ are resource invariant in relation to $\Delta, \Delta_1, ..., \Delta_n, \Xi$ \\
2.5 \hspace{2cm} $\mz p; p \rightarrow p$, $\mz \Delta_1; \Omega'_1 \rightarrow \Delta_1$ ... $\mz \Delta_k; \Omega'_k \rightarrow \Delta_k$ and $\mz \Xi_1; \Lambda_1 \rightarrow \Xi_1$ ... $\mz \Xi_m; \Lambda_m \rightarrow \Xi_m$\\

\end{itemize}

\begin{proof}
   By nested induction. In $\mc$ on the size of $\Omega = \Omega_1, ..., \Omega_n$. In $\contc$, first on the size of $\Delta''$ of the continuation frame and then on the continuation stack $C$.
   
   \begin{itemize}
      \item $\mc p \; ok \; first$
      
      By induction on $\Omega$.\\
      Stack frame $(\Delta, p_1; \Delta''; \Xi; p; \Omega; \cdot)$ is flat well-formed. \\
      
      \item $\mc p \; ok \; other$
      
      By induction on $\Omega$.\\
      Stack frame $(\Delta, p_1; \Delta''; \Xi; p; \Omega; q, \Lambda)$ is flat well-formed.
      
      \item $\mc p \; fail$
      
      By mutual induction on $\contc$.
      
      \item $\mc \otimes$
      
      By induction on $\Omega$. \\
      
      \item $\mc end$
      
      Select case 2 with assumption.
      
      \item $\contc end$
      
      Select case 1 with assumption.
      
      \item $\contc next$
      
      By induction on $\Delta''$.\\
      
      \item $\contc next \; empty$
      
      By induction on the size of $C$.
      
   \end{itemize}
\end{proof}

\subsubsection{Comprehension soundness lemma}

If $\mc \Delta, \Xi; \Xi_N; \Delta_{N1}; \cdot; A; \cdot; \comp A \lolli B; \Omega_N; \Delta_N \rightarrow \Xi'; \Delta'$ where $\Delta, \Xi = \Delta_N$ then either:\\
1. \hspace{1cm} $\done \Delta_N; \Xi_N; \Delta_{N1}; \Omega_N \rightarrow \Xi'; \Delta'$ or \\
2. \hspace{1cm} $\mc \Delta; \Xi_N; \Delta_{N1}; \Xi; \cdot; C'; \comp A \lolli B; \Omega_N; \Delta_N \rightarrow \Xi'; \Delta'$ and \\
2.1 \hspace{2cm} $\mz \Delta_1; A \rightarrow \Delta_1$ \\
2.2 \hspace{2cm} $C'$ is flat well-formed in relation to $A$. \\
2.3 \hspace{2cm} $C'$ is resource invariant in relation to $\Delta, \Xi$ \\

\begin{proof}
Direct application of the previous theorem.
\end{proof}

\subsubsection{Dall transformation theorem}

If $\dall \Xi_N; \Delta_{N1}; \Xi; C, (\Delta_a; \Delta_b; \cdot; \Omega; \cdot); \comp A \lolli B; \Omega_N; \Delta_N \rightarrow \Xi'; \Delta'$ then\\
$\dc \Xi_N, \Xi; \Delta_{N1}; B; (\Delta_a - \Xi; \Delta_b - \Xi; \cdot; \Omega; \cdot); \comp A \lolli B; \Omega_N; (\Delta_N - \Xi) \rightarrow \Xi'; \Delta'$.

\begin{proof}
   By induction on the size of the continuation stack $C$.
   
   \begin{itemize}
      \item $C = \_, X, C'$
      
      $\dall \Xi_N; \Delta_{N1}; \Xi; \_, X, C'; \comp A \lolli B; \Omega_N; \Delta_N \rightarrow \Xi'; \Delta'$ \hfill (1) assumption \\
      $\dall \Xi_N; \Delta_{N1}; \Xi; X, C'; \comp A \lolli B; \Omega_N; \Delta_N \rightarrow \Xi'; \Delta'$ \hfill (2) inversion of (1) \\
      $\dc \Xi_N, \Xi; \Delta_{N1}; B; (\Delta_a - \Xi; \Delta_b - \Xi; \cdot; \Omega; \cdot); \comp A \lolli B; \Omega_N; (\Delta_N - \Xi) \rightarrow \Xi'; \Delta'$ \hfill (3) i.h. on (2) \\
      
      \item $C = (\Delta_a - \Xi; \Delta_b - \Xi; \cdot; \Omega; B)$
      
      $\dall \Xi_N; \Delta_{N1}; \Xi; (\Delta_a; \Delta_b; \cdot; \Omega; \cdot); \comp A \lolli B; \Omega_N; \Delta_N \rightarrow \Xi'; \Delta'$ \hfill (1) assumption \\
      $\dc \Xi_N, \Xi; \Delta_{N1}; B; (\Delta_a - \Xi; \Delta_b - \Xi; \cdot; \Omega; B); \comp A \lolli B; \Omega_N; (\Delta_N - \Xi) \rightarrow \Xi'; \Delta'$ \hfill (2) inversion of (1) \\
   \end{itemize}
\end{proof}

\subsubsection{Successful comprehension match gives derivation}

If $\mc \Delta; \Xi_N; \Delta_{N1}; \Xi; \cdot; B; C, (\Delta_a; \Delta_b; \cdot; p; \Omega; \cdot); \comp A \lolli B; \Omega_N; \Delta_N \rightarrow \Xi'; \Delta'$ then:\\
\hspace{1cm} $\dc \Xi_N, \Xi; \Delta_{N1}; B; (\Delta_a - \Xi; \Delta_b - \Xi; \cdot; p; \Omega; \cdot); \comp A \lolli B; \Omega_N; (\Delta_N - \Xi) \rightarrow \Xi'; \Delta'$.

\begin{proof}
   Invert the assumption and then apply dall transformation theorem.
\end{proof}

\subsubsection{Continuation derivation theorem}

If $\dc \Xi_N; \Delta_{N1}; \Omega_1, ..., \Omega_n; C; \comp A \lolli B; \Omega_N; \Delta_N \rightarrow \Xi'; \Delta'$ then:\\
1. \hspace{1cm} $\dc \Xi_N; \Delta_{N1}, \Delta_1, ..., \Delta_n; \cdot; C; \comp A \lolli B; \Omega_N; \Delta_N \rightarrow \Xi'; \Delta'$ and \\
2. \hspace{1cm} If $\dz \Delta; \Xi_N; \Delta_{N1}, \Delta_1, ..., \Delta_n; \Omega \rightarrow \Xi'; \Delta'$ then $\dz \Delta; \Xi_N; \Delta_{N1}; \Omega_1, ..., \Omega_n, \Omega \rightarrow \Xi'; \Delta'$

\begin{proof}
   By induction on the size of $\Omega_1, ..., \Omega_n$.
   
   \begin{itemize}
      \item $p, \Omega$
      
      $\dc \Xi_N; \Delta_{N1}; p, \Omega_2, ..., \Omega_n; C; \comp A \lolli B; \Omega_N; \Delta_N \rightarrow \Xi'; \Delta'$ \hfill (1) assumption \\
      $\dc \Xi_N; \Delta_{N1}, p; \Omega_2, ..., \Omega_n; C; \comp A \lolli B; \Omega_N; \Delta_N \rightarrow \Xi'; \Delta'$ \hfill (2) inversion of (1) \\
      $\dc \Xi_N; \Delta_{N1}, p, \Delta_2, ..., \Delta_n; \cdot; C; \comp A \lolli B; \Omega_N; \Delta_N \rightarrow \Xi'; \Delta'$ \hfill (3) i.h. on (2) \\
      if $\dz \Delta; \Xi_N; \Delta_{N1}, p, \Delta_2, ..., \Delta_n; \Omega \rightarrow \Xi'; \Delta'$ then $\dz \Delta; \Xi_N; \Delta_{N1}; p, \Omega_2, ..., \Omega_n, \Omega \rightarrow \Xi'; \Delta'$ \hfill (4) i.h. on (2) \\
      $\dz \Delta; \Xi_N; \Delta_{N1}, p, \Delta_2, ..., \Delta_n; \Omega \rightarrow \Xi'; \Delta'$ \hfill (5) from (4) \\
      $\dz \Delta; \Xi_N; \Delta_{N1}; p, \Omega_2, ..., \Omega_n, \Omega \rightarrow \Xi'; \Delta'$ \hfill (6) using (5) on (4) \\
      
      \item $1, \Omega$
      
      By induction.
      
      \item $A \otimes B, \Omega$
      
      $\dc \Xi_N; \Delta_{N1}; A \otimes B, \Omega_2, ..., \Omega_n; C; \comp A \lolli B; \Omega_N; \Delta_N \rightarrow \Xi'; \Delta'$ \hfill (1) assumption \\
      $\dc \Xi_N; \Delta_{N1}; A, B, \Omega_2, ..., \Omega_n; C; \comp A \lolli B; \Omega_N; \Delta_N \rightarrow \Xi'; \Delta'$ \hfill (2) inversion of (1) \\
      Solve by induction on (2) \\
   \end{itemize}
\end{proof}

\subsubsection{Continuation derivation lemma}

If $\dc \Xi_N; \Delta_{N1}; \Omega_x; C; \comp A \lolli B; \Omega_N; \Delta_N \rightarrow \Xi'; \Delta'$ then: \\
1. \hspace{1cm} $\dc \Xi_N; \Delta_{N1}, \Delta_x; \cdot; C; \comp A \lolli B; \Omega_N; \Delta_N \rightarrow \Xi'; \Delta'$ and \\
2. \hspace{1cm} If $\dz \Delta; \Xi_N; \Delta_{N1}, \Delta_x; \Omega \rightarrow \Xi'; \Delta'$ then $\dz \Delta; \Xi_N; \Delta_{N1}; \Omega_x, \Omega \rightarrow \Xi'; \Delta'$

\begin{proof}
   By direct application of the continuation derivation theorem.
\end{proof}

\subsubsection{Comprehension Theorem}

If $\mc \Delta_a, \Delta'_b; \Xi_N; \Delta_{N1}; p_1; \Omega; (\Delta_a, p_1; \Delta'_b; \cdot; p; \Omega; \cdot); \comp A \lolli B; \Omega_N; \Delta, \Xi_1, ..., \Xi_n \rightarrow \Xi'; \Delta'$ and $\Delta_a, \Delta_b = \Delta, \Xi_1, ..., \Xi_n$ and $\feq{p, \Omega}{A}$ then $\exists n \geq 0$ such that: \\
1. \hspace{1cm} $\done \Delta; \Xi_N, \Xi_1, ..., \Xi_n; \Delta_{N1}, \Delta_1, ..., \Delta_n; \Omega_N \rightarrow \Xi'; \Delta'$\\
2. \hspace{1cm} $\mz \Xi_1; A \rightarrow \Xi_1$ ... $\mz \Xi_n; A \rightarrow \Xi_n$ \\
3. \hspace{1cm} $n$ implications from $1 ... i ... n$ such that: $\forall \Omega_x, \Delta_x.$ if $\dz \Delta_x; \Xi_N, \Xi_1, ..., \Xi_i; \Delta_{N1}, \Delta_1, ..., \Delta_i; \Omega_x \rightarrow \Xi'; \Delta'$ then $\dz \Delta_x; \Xi_N, \Xi_1, ..., \Xi_i; \Delta_{N1}, \Delta_1, ..., \Delta_{i-1}; B, \Omega_x \rightarrow \Xi'; \Delta'$.

\begin{proof}
   By induction on the size of $\Delta_b$.\\

   $\Delta_b = p_1, \Delta'_b$ \hfill (1) from assumption \\
   $\Delta_a, p_1, \Delta'_b = \Delta, p, \Xi'_1, ..., \Xi_n$ \hfill (2) from assumption \\
   By applying the comprehension soundness theorem on the assumption:\\
      
   \begin{itemize}
      \item Failure:
         
      $\done \Delta, \Xi_1, ..., \Xi_n; \Xi_N; \Delta_{N1}; \Omega_N \rightarrow \Xi'; \Delta'$ \hfill (3) assumption (so $n = 0$)\\
         
      \item Success:
         
      $\mc \Delta, \Xi_2, ..., \Xi_n; \Xi_N; \Delta_{N1}; p, \Xi'_1; \cdot; C', (\Delta_a, p_1; \Delta'_b; \cdot; p; \Omega; \cdot); \comp A \lolli B; \Omega_N; \Delta, \Xi_1, ..., \Xi_n \rightarrow \Xi'; \Delta'$ \hfill (3) assumption \\
      $\mz p_1; p \rightarrow p_1$ and $\mz \Xi'_1; \Omega \rightarrow \Xi'_1$ \hfill (4) assumption \\
      $C'$ is flat well-formed \hfill (5) assumption \\
      $\mz p_1, \Xi'_1; p \otimes \Omega \rightarrow p_1, \Xi'_1$ \hfill (6) from (4) \\
      $\feq{p, \Omega}{A}$ \hfill (7) assumption about the original continuation stack \\
      $\mz p_1, \Xi'_1; A \rightarrow p_1, \Xi'_1$ \hfill (8) from match equivalence theorem on (6) and (7) \\
      $\dc \Xi_N, p, \Xi'_1; \Delta_{N1}; B; (\Delta_a, p_1 - (p_1, \Xi'_1); \Delta'_b - (p_1, \Xi'_1); \cdot; p; \Omega; \cdot); \comp A \lolli B; \Omega_N; (\Delta, \Xi_1, ..., \Xi_n) - \Xi_1 \rightarrow \Xi'; \Delta'$ \hfill (9) apply successful comprehension matches gives derivation lemma to (3) \\
      $\dc \Xi_N, p, \Xi'_1; \Delta_{N1}; B; (\Delta_a - \Xi'_1; \Delta'_b - \Xi'_1; \cdot; p; \Omega; \cdot); \comp A \lolli B; \Omega_N; \Delta, \Xi_2, ..., \Xi_n \rightarrow \Xi'; \Delta'$ \hfill (10) simplification of (9) \\
      $\dc \Xi_N, p, \Xi'_1; \Delta_{N1}, \Delta_1; \cdot; (\Delta_a - \Xi'_1; \Delta'_b - \Xi'_1; \cdot; p; \Omega; \cdot); \comp A \lolli B; \Omega_N; \Delta, \Xi_2, ..., \Xi_n \rightarrow \Xi'; \Delta'$ \hfill (11) from continuation derivation lemma on (10)\\
      if $\forall \Omega_x, \Delta_x. \dz \Delta_x; \Xi_N, p, \Xi'_1; \Delta_{N1}, \Delta_1; \Omega_x \rightarrow \Xi'; \Delta'$ then $\dz \Delta_x; \Xi_N, p, \Xi'_1; \Delta_{N1}; B, \Omega_x \rightarrow \Xi'; \Delta'$ \hfill (12) using the same lemma \\
      $\contc \Delta, \Xi_2, ..., \Xi_n; \Xi_N, p, \Xi'_1; \Delta_{N1}, \Delta_1; (\Delta_a - \Xi'_1; \Delta'_b - \Xi'_1; \cdot; p; \Omega; \cdot); \comp A \lolli B; \Omega_N \rightarrow \Xi'; \Delta'$ \hfill (13) inversion of (11) \\   
      
      When inverting (11), we have two subcases:
      
      $\Delta_a - \Xi'_1 = \Delta''_a$ \hfill (12) \\
      $\Delta'_b - \Xi'_1 = \Delta''_b$ \hfill (13) \\
      $\Delta''_a, \Delta''_b = \Delta, \Xi_2, ..., \Xi_n$ \hfill (14) \\
      
      \begin{itemize}
         \item End ($n = 1$):
         
         $\contc \Delta, \Xi_2, ..., \Xi_n; \Xi_N, \Xi_1; \Delta_{N1}, \Delta_1; \cdot; \comp A \lolli B; \Omega_N \rightarrow \Xi'; \Delta'$ \hfill (15) \hfill inversion of (11) \\
         $\done \Delta, \Xi_2, ..., \Xi_n; \Xi_N, \Xi_1; \Delta_{N1}, \Delta_1; \Omega_N \rightarrow \Xi'; \Delta'$ \hfill (16) inverting (15), which is what we want \\
         
         \item Next ($n = n' + 1$):
         
         $\Delta'''_b = \Delta''_b, p_2$ \hfill (15) from inversion \\
         $\mc \Delta''_a, \Delta'''_b; \Xi_N, \Xi_1; \Delta_{N1}, \Delta_1; \cdot; \Omega; (\Delta''_a, p_2; \Delta'''_b; \cdot; p; \Omega; \cdot); \comp A \lolli B; \Omega_N; \Delta, \Xi_2, ..., \Xi_n \rightarrow \Xi'; \Delta'$ \hfill (16) inversion of (11) \\
         Apply induction hypotheses to (16) to get results from $n'$.\\ 
      \end{itemize}
      
      \item Backtrack:
      
      $f = (\Delta_a, p_1; \Delta'_b; \cdot; p; \Omega; \cdot)$ \hfill (3) from theorem \\
      turns into $f' = (\Delta_a, p_1, \Delta'''_b, p_2; \Delta''_b; \cdot; p; \Omega; \cdot)$ \hfill (4) from theorem (3) \\
      $\mc \Delta, \Xi_2, ..., \Xi_n; \Xi_N; \Delta_{N1}; p_2, \Xi'_1; \cdot; C', f'; \comp A \lolli B; \Omega_N; \Delta, \Xi_1, ..., \Xi_n \rightarrow \Xi'; \Delta'$ \hfill (5) from theorem (3) \\
      $\mz p_2; p \rightarrow p_2$ \hfill (6) from theorem (3) \\
      $\mz \Xi'_1; \Omega \rightarrow \Xi'_1$ \hfill (7) from theorem (3) \\
      $\mz p_2, \Xi'_1; \Omega \otimes p \rightarrow p_2, \Xi'_1$ \hfill (8) rule application on (6) and (7) \\
      $\feq{p, \Omega}{A}$ \hfill (9) from assumptions \\
      $\mz p_2, \Xi'_1 ; A \rightarrow p_2, \Xi'_1$ \hfill (10) using match equivalence theorem \\
      
      Use the same approach as the last subcase, but using $p_2$ instead of $p_1$ and using the fact that $\Delta_b$ was already reduced because we had to backtrack.
   \end{itemize}
   
   
\end{proof}

\subsubsection{Comprehension Lemma}

If $\mc \Delta, \Xi_1, ..., \Xi_n; \Xi_N; \Delta_{N1}; \cdot; A; \cdot; \comp A \lolli B; \Omega_N; \Delta, \Xi_1, ..., \Xi_n \rightarrow \Xi'; \Delta'$ then we can apply the comprehension $n >= 0$ times: \\
1. \hspace{1cm} $\done \Delta; \Xi_N, \Xi_1, ..., \Xi_n; \Delta_{N1}, \Delta_1, .., \Delta_n; \Omega_N \rightarrow \Xi'; \Delta'$ for $\exists n \geq 0$\\
2. \hspace{1cm} $\mz \Xi_1; A \rightarrow \Xi_1$ ... $\mz \Xi_n; A \rightarrow \Xi_n$.\\
3. \hspace{1cm} $n$ implications from $1 ... i ... n$ such that: $\forall \Omega_x, \Delta_x.$ if $\dz \Delta_x; \Xi_N, \Xi_1, ..., \Xi_i; \Delta_{N1}, \Delta_1, ..., \Delta_i; \Omega_x \rightarrow \Xi'; \Delta'$ then $\dz \Delta_x; \Xi_N, \Xi_1, ..., \Xi_i; \Delta_{N1}, \Delta_1, ..., \Delta_{i-1}; B, \Omega_x \rightarrow \Xi'; \Delta'$.

\begin{proof}
   Applying the comprehension soundness lemma, we get two cases:
   
   \begin{itemize}
      \item Failure:
      
      $\done \Delta, \Xi_1, ..., \Xi_n; \Xi_N; \Delta_{N1}; \Omega_N \rightarrow \Xi'; \Delta'$ \hfill no comprehension application was possible.
      
      \item Success:
      
      $\mc \Delta, \Xi_2, ..., \Xi_n; \Xi_N; \Delta_{N1}; \Xi_1; \cdot; C'; \comp A \lolli B; \Omega_N; \Delta, \Xi_1, ..., \Xi_n \rightarrow \Xi'; \Delta'$ \hfill (1) result from theorem \\
      $\mz \Xi_1; A \rightarrow \Xi_1$ \hfill (2) from theorem \\
      $C$ is flat well-formed in relation to $A$. \hfill (3) from theorem \\
      $C$ is resource invariant in relation to $\Delta, \Xi_1, ..., \Xi_n$ \hfill (4) from theorem \\
      
      $\dc \Xi_N, \Xi_1; \Delta_{N1}; B; (\Delta_a - \Xi_1; \Delta_b - \Xi_1; \cdot; p; \Omega; \cdot); \comp A \lolli B; \Omega_N; (\Delta, \Xi_1, ..., \Xi_n - \Xi_1) \rightarrow \Xi'; \Delta'$ \hfill (5) applying successful comprehension match gives derivation \\
      $\dc \Xi_N, \Xi_1; \Delta_{N1}; B; (\Delta_a - \Xi_1; \Delta_b - \Xi_1; \cdot; p; \Omega; \cdot); \comp A \lolli B; \Omega_N; \Delta, \Xi_2, ..., \Xi_n \rightarrow \Xi'; \Delta'$ \hfill (6) simplifying (5) \\
      $\Delta_a, \Delta_b = \Delta, \Xi_1, ..., \Xi_n$ \hfill (7) from (4) \\
      $(\Delta_a - \Xi_1), (\Delta_b - \Xi_1) = (\Delta_a, \Delta_b) - \Xi_1 = \Delta_, \Xi_2, .., \Xi_n$ and $\Delta'_a = \Delta_a - \Xi_1$ and $\Delta'_b = \Delta_b - \Xi_1$ \hfill (8) from (7) and (6) \\
      $\feq{p, \Omega}{A}$ \hfill (9) from (3) and (6) \\
      $\dc \Xi_N, \Xi_1; \Delta_{N1}, \Delta_1; (\Delta'_a; \Delta'_b; \cdot; p; \Omega; \cdot); \comp A \lolli B; \Omega_N; \Delta, \Xi_2, ..., \Xi_n \rightarrow \Xi'; \Delta'$ \hfill (10) using continuation derivation lemma \\
      if $\forall \Omega_x, \Delta_x. \dz \Delta_x; \Xi_N, \Xi_1; \Delta_{N1}, \Delta_1; \Omega_x \rightarrow \Xi'; \Delta'$ then $\dz \Delta_x; \Xi_N, \Xi_1; \Delta_{N1}; B, \Omega_x \rightarrow \Xi'; \Delta'$ \hfill (11) using the same lemma \\ 
      $\contc \Delta, \Xi_2, ..., \Xi_n; \Xi_N, \Xi_1; \Delta_{N1}, \Delta_1; (\Delta'_a; \Delta'_b; \cdot; p; \Omega; \cdot); \comp A \lolli B; \Omega_N \rightarrow \Xi'; \Delta'$ \hfill (12) inversion of (10) \\
      Apply continuation theorem to (12) to get the remaining $n-1$.
   \end{itemize}
\end{proof}

\subsubsection{Body Derive Soundness}

If $\done \Delta; \Xi; \Delta_1; \Omega \rightarrow \Xi'; \Delta$ then $\dz \Delta; \Xi; \Delta_1; \Omega \rightarrow \Xi'; \Delta'$.

\begin{proof}
   By induction on $\Omega$.
   
   \begin{itemize}
      \item $p, \Omega$
      
      By induction.
      
      \item $1, \Omega$
      
      By induction.
      
      \item $A \otimes B, \Omega$
      
      By induction.
      
      \item $\cdot$
      
      Use axiom.
      
      \item $\comp A \lolli B, \Omega$
      
      By using the comprehension lemma, we get $n$ applications of the comprehension.\\
      $\Delta = \Delta, \Xi_1, ..., \Xi_n$ \hfill (1)\\
      $\done \Delta; \Xi, \Xi_1, ..., \Xi_n; \Delta_1, \Delta_{c_1}, ..., \Delta_{c_n}; \Omega \rightarrow \Xi'; \Delta'$ \hfill (2) from lemma \\
      $\dz \Delta; \Xi, \Xi_1, ..., \Xi_n; \Delta_1, \Delta_{c_1}, ..., \Delta_{c_n}; \Omega \rightarrow \Xi'; \Delta'$ \hfill (3) i.h. on (2) \\
      $\dz \Delta; \Xi, \Xi_1, ..., \Xi_n; \Delta_1, \Delta_{c_1}, ..., \Delta_{c_n}; 1, \Omega \rightarrow \Xi'; \Delta'$ \hfill (4) apply $\dz 1$ on (3) \\
      $\dz \Delta; \Xi, \Xi_1, ..., \Xi_n; \Delta_1, \Delta_{c_1}, ..., \Delta_{c_n}; 1 \with (A \lolli B \otimes \comp A \lolli B), \Omega \rightarrow \Xi'; \Delta'$ \hfill (5) apply $\dz \with L$ on (4) \\
      $\dz \Delta; \Xi, \Xi_1, ..., \Xi_n; \Delta_1, \Delta_{c_1}, ..., \Delta_{c_n}; \comp A \lolli B, \Omega \rightarrow \Xi'; \Delta'$ \hfill (6) apply $\dz comp$ on (5) \\
      Using the $n^{th}$ implication of the comprehension theorem:\\
      $\dz \Delta; \Xi, \Xi_1, ..., \Xi_n; \Delta_1, \Delta_{c_1}, ..., \Delta_{c_{n-1}}; B, \comp A \lolli B, \Omega \rightarrow \Xi'; \Delta'$ \hfill (7) \\
      Using the $\mz \Xi_n; A \rightarrow \Xi_n$ result: \\
      $\dz \Delta, \Xi_n; \Xi_1, ..., \Xi_{n-1}; \Delta_1, \Delta_{c_1}, ..., \Delta_{c_{n-1}}; A \lolli B, \comp A \lolli B, \Omega \rightarrow \Xi'; \Delta'$ \hfill (8) using $\mz$ on (7) \\
      $\dz \Delta, \Xi_n; \Xi_1, ..., \Xi_{n-1}; \Delta_1, \Delta_{c_1}, ..., \Delta_{c_{n-1}}; A \lolli B \otimes \comp A \lolli B, \Omega \rightarrow \Xi'; \Delta'$ \hfill (9) applying rule $\dz \otimes$ on (8) \\
      $\dz \Delta, \Xi_n; \Xi_1, ..., \Xi_{n-1}; \Delta_1, \Delta_{c_1}, ..., \Delta_{c_{n-1}}; 1 \with (A \lolli B \otimes \comp A \lolli B), \Omega \rightarrow \Xi'; \Delta'$ \hfill (10) applying rule $\dz \with R$ on (9) \\
      $\dz \Delta, \Xi_n; \Xi_1, ..., \Xi_{n-1}; \Delta_1, \Delta_{c_1}, ..., \Delta_{c_{n-1}}; \comp A \lolli B, \Omega \rightarrow \Xi'; \Delta'$ \hfill (11) applying rule $\dz comp$ on (10) \\
      By applying the other $n-1$ comprehensions we will get: \\
      $\dz \Delta, \Xi_1, ..., \Xi_n; \Delta_1; \comp A \lolli B, \Omega \rightarrow \Xi'; \Delta'$ \hfill (12)
   \end{itemize}
\end{proof}